theories/Syntax/Typ.v
@@ -19,15 +19,15 @@ Open Scope resources_scope.
 
 Module RS := Resources.
 
-(** **** Type
+(** **** The set of types
 
-  A type is either a ground type, named [unit], a function type, a product type or a reactive type, also named signal function type. The first three type are usual in the extended lambda-calculus. The last one is a type taken from the arrow-calculus and represent reactive expressions. In addition, it carries a set of resource names representing interaction with the environment done by the expression.
+  A type is either a ground type, named [unit], a function type, a product type or a reactive type, also named signal function type. The first three types are usual in the extended lambda-calculus. The last one is a type taken from the arrow-calculus and represent reactive expressions. In addition, it carries a set of resource names representing interaction with the environment done by the expression.
 *)
-Inductive raw : Type :=
-  | ty_unit : raw
-  | ty_arrow (α β : raw) : raw
-  | ty_prod  (α β : raw) : raw
-  | ty_reactive (α β : raw) (R : resources) : raw
+Inductive raw: Type :=
+  | ty_unit: raw
+  | ty_arrow (α β: raw): raw
+  | ty_prod  (α β: raw): raw
+  | ty_reactive (α β: raw) (R: resources): raw
 .
 
 Definition t := raw.
@@ -35,9 +35,9 @@ Definition eq := @Logic.eq t.
 
 (** **** Shift function 
 
-  The shift function impacts only the set of used resources. It takes a type goes through all sub-terms and applies the shift function defined for sets, in [Levels], on all used resource sets encountered. It is denoted [[⧐ _ – _] _].
+  The shift function impacts only resource sets carried by signal function types. It takes a type goes through all sub-terms and applies the shift function defined for sets, in [Levels], on all resource sets encountered. It is denoted [[⧐ _ – _] _].
 *)
-Fixpoint shift (lb : lvl) (k : lvl) (α : t) : t := 
+Fixpoint shift (lb: lvl) (k: lvl) (α: t): t := 
   match α with
     | ty_arrow t1 t2 => ty_arrow (shift lb k t1) (shift lb k t2)    
     | ty_prod  t1 t2 => ty_prod  (shift lb k t1) (shift lb k t2)    
@@ -50,44 +50,43 @@ Fixpoint shift (lb : lvl) (k : lvl) (α : t) : t :=
 
   As done in [Resource.v] and [Resources.v], we define a [multi_shift] function that applies [n] shifts for two lists [lbs] and [ks] of length [n].
 *)
-Definition multi_shift (lbs : list lvl) (ks : list lvl) (α : t) :=
+Definition multi_shift (lbs: list lvl) (ks: list lvl) (α: t) :=
   List.fold_right (fun lbk acc => shift (fst lbk) (snd lbk) acc) α (List.combine lbs ks).
 
 
 (** **** Well-formedness
 
-  The well-formed property, named [Wf] and denoted [(⊩)], takes a level [k] called the well-formedness level and states that all resource names in the type are well-formed under [k]. Recall that a resource name [r] is well-formed under [k] if [r < k] and a resource set [s] is well-formed under [k] if all
-  [r] in [s] are well-formed under [k].
+  The well-formed property, named [Wf] and denoted [(⊩)], takes a level [k] called the well-formedness level and states that all resource names in the type are well-formed under [k]. Recall that a resource name [r] is well-formed under [k] if [r < k] and a resource set [s] is well-formed under [k] if all [r] in [s] are well-formed under [k].
 *)
-Inductive Wf' : lvl -> t -> Prop :=
-  | vΤ_unit (k : lvl): Wf' k ty_unit
-  | vΤ_prod (k : lvl) (α β : t): Wf' k α -> Wf' k β -> Wf' k (ty_prod α β)
-  | vΤ_func (k : lvl) (α β : t): Wf' k α -> Wf' k β -> Wf' k (ty_arrow α β)
-  | vΤ_reac (k : lvl) (α β : t) (R : resources): 
+Inductive Wf': lvl -> t -> Prop :=
+  | vΤ_unit (k: lvl): Wf' k ty_unit
+  | vΤ_prod (k: lvl) (α β: t): Wf' k α -> Wf' k β -> Wf' k (ty_prod α β)
+  | vΤ_func (k: lvl) (α β: t): Wf' k α -> Wf' k β -> Wf' k (ty_arrow α β)
+  | vΤ_reac (k: lvl) (α β: t) (R: resources): 
                    Wf' k α -> Wf' k β -> k ⊩ R -> Wf' k (ty_reactive α β R)
 .
 
 Definition Wf := Wf'.
 
-#[export] Hint Constructors Wf' : core.
+#[export] Hint Constructors Wf': core.
 
 (** *** Properties *)
 
 (** **** [eq] properties *)
 
-#[export] Instance eq_refl : Reflexive eq := _.
+#[export] Instance eq_refl: Reflexive eq := _.
 
-#[export] Instance eq_sym : Symmetric eq := _.
+#[export] Instance eq_sym: Symmetric eq := _.
 
-#[export] Instance eq_trans : Transitive eq := _.
+#[export] Instance eq_trans: Transitive eq := _.
 
-#[export] Instance eq_equiv : Equivalence eq := _.
+#[export] Instance eq_equiv: Equivalence eq := _.
 
-#[export] Instance eq_rr : RewriteRelation eq := {}.
+#[export] Instance eq_rr: RewriteRelation eq := {}.
 
-#[export] Hint Resolve eq_refl eq_sym eq_trans : core.
+#[export] Hint Resolve eq_refl eq_sym eq_trans: core.
 
-Lemma eq_dec (α β : t): {eq α β} + {~ eq α β}.
+Lemma eq_dec (α β: t): {eq α β} + {~ eq α β}.
 Proof.
   unfold eq; revert β; induction α; intro; destruct β; simpl; auto; 
   try (right; unfold not; intros contra; now inversion contra).
@@ -103,31 +102,31 @@ Proof.
     -- right; unfold not in *; intros; inversion H; subst; apply n; reflexivity.
 Qed.
 
-Lemma eq_dec' (α β : t): {α = β} + {α <> β}.
+Lemma eq_dec' (α β: t): {α = β} + {α <> β}.
 Proof. apply eq_dec. Qed.
 
-Lemma eq_leibniz (α β : t): eq α β -> α = β. 
+Lemma eq_leibniz (α β: t): eq α β -> α = β. 
 Proof. auto. Qed.
 
 (** **** [shift] properties *)
 
-Lemma shift_zero_refl (k : lvl) (α : t):
+Lemma shift_zero_refl (k: lvl) (α: t):
   (shift k 0 α) = α.
 Proof.
   induction α; simpl; f_equal; auto.
   apply RS.eq_leibniz; apply RS.shift_zero_refl.
 Qed.
 
-Lemma shift_wf_refl (lb k : lvl) (α : t):
+Lemma shift_wf_refl (lb k: lvl) (α: t):
   Wf lb α -> shift lb k α = α.
 Proof.
   intro Hv; induction Hv; subst; simpl; f_equal; auto.
   apply RS.eq_leibniz; now apply RS.shift_wf_refl.
 Qed.
 
-#[export] Instance shift_eq : Proper (Logic.eq ==> Logic.eq ==> eq ==> eq) shift := _.
+#[export] Instance shift_eq: Proper (Logic.eq ==> Logic.eq ==> eq ==> eq) shift := _.
 
-Lemma shift_eq_iff (lb k : lvl) (α β : t):
+Lemma shift_eq_iff (lb k: lvl) (α β: t):
   α = β <-> (shift lb k α) = (shift lb k β).
 Proof.
   split; intro Heq.
@@ -139,35 +138,35 @@ Proof.
     now rewrite H2.
 Qed.
 
-Lemma shift_trans (lb m n : lvl) (α : t):
+Lemma shift_trans (lb m n: lvl) (α: t):
   shift lb m (shift lb n α) = shift lb (m + n) α.
 Proof.
   induction α; simpl; f_equal; auto.
   apply RS.eq_leibniz; apply RS.shift_trans.
 Qed.
 
-Lemma shift_permute (lb m n : lvl) (α : t):
+Lemma shift_permute (lb m n: lvl) (α: t):
   shift lb m (shift lb n α) = shift lb n (shift lb m α).
 Proof.
   induction α; simpl; f_equal; auto.
   apply RS.eq_leibniz; apply RS.shift_permute.
 Qed.
 
-Lemma shift_permute_1 (lb m n : lvl) (α : t):
+Lemma shift_permute_1 (lb m n: lvl) (α: t):
   eq (shift lb m (shift lb n α)) (shift (lb + m) n (shift lb m α)).
 Proof.
   unfold eq; induction α; intros; simpl; f_equal; auto.
   apply RS.eq_leibniz; apply RS.shift_permute_1.
 Qed.
 
-Lemma shift_permute_2 (lb k m n : lvl) (α : t):
+Lemma shift_permute_2 (lb k m n: lvl) (α: t):
   lb <= k -> eq (shift lb m (shift k n α)) (shift (k + m) n (shift lb m α)).
 Proof.
   unfold eq; induction α; intros; simpl; f_equal; auto.
   apply RS.eq_leibniz; now apply RS.shift_permute_2.
 Qed.
 
-Lemma shift_unfold (lb m n : lvl) (α : t):
+Lemma shift_unfold (lb m n: lvl) (α: t):
   eq (shift lb (m + n) α) (shift (lb + m) n (shift lb m α)). 
 Proof.
   induction α; simpl; auto; try now rewrite IHα1; rewrite IHα2.
@@ -176,7 +175,7 @@ Proof.
   now apply RS.shift_unfold.
 Qed.
 
-Lemma shift_unfold_1 (k m n : lvl) (α : t):
+Lemma shift_unfold_1 (k m n: lvl) (α: t):
   k <= m -> m <= n -> eq (shift m (n - m) (shift k  (m - k) α)) (shift k (n - k) α).
 Proof.
   induction α; simpl; intros Hlekm Hlemn; auto; 
@@ -188,16 +187,16 @@ Qed.
 
 (** **** [Wf] properties *)
 
-#[export] Instance Wf_iff : Proper (Logic.eq ==> eq ==> iff) Wf := _.
+#[export] Instance Wf_iff: Proper (Logic.eq ==> eq ==> iff) Wf := _.
 
-Lemma Wf_weakening (k n : lvl) (α : t): (k <= n) -> Wf k α -> Wf n α.
+Lemma Wf_weakening (k n: lvl) (α: t): (k <= n) -> Wf k α -> Wf n α.
 Proof.
   unfold Wf; induction α; intros Hleq Hvτ; simpl in *; inversion Hvτ; subst; eauto.
   apply vΤ_reac; eauto. 
   eapply RS.Wf_weakening; eauto.
 Qed.
 
-Theorem shift_preserves_wf_1 (k m n : lvl) (α : t):
+Theorem shift_preserves_wf_1 (k m n: lvl) (α: t):
   Wf m α -> Wf (m + n) (shift k n α).
 Proof.
   unfold Wf; induction α; intro Hvτ; inversion Hvτ; subst; simpl; auto.
@@ -205,17 +204,17 @@ Proof.
   now apply RS.shift_preserves_wf_1.
 Qed.
 
-Theorem shift_preserves_wf (m n : lvl) (α : t):
+Theorem shift_preserves_wf (m n: lvl) (α: t):
   Wf m α -> Wf (m + n) (shift m n α).
 Proof. now apply shift_preserves_wf_1. Qed.
 
-Lemma shift_preserves_wf_zero (k : lvl) (α : t): Wf k α -> Wf k (shift k 0 α).
+Lemma shift_preserves_wf_zero (k: lvl) (α: t): Wf k α -> Wf k (shift k 0 α).
 Proof. 
   intro Hvα; replace k with (k + 0) by auto. 
   now apply shift_preserves_wf_1. 
 Qed.
 
-Lemma shift_preserves_wf_gen (lb k m n : lvl) (α : t):
+Lemma shift_preserves_wf_gen (lb k m n: lvl) (α: t):
   m <= n -> lb <= k -> m <= lb -> n <= k -> n - m = k - lb -> 
   Wf lb α -> Wf k (shift m (n - m) α).
 Proof.
@@ -224,7 +223,7 @@ Proof.
   apply RS.shift_preserves_wf_gen with lb; auto.
 Qed.
 
-Lemma shift_preserves_wf_2 (m n : lvl) (α : t):
+Lemma shift_preserves_wf_2 (m n: lvl) (α: t):
   m <= n -> Wf m α -> Wf n (shift m (n - m) α).
 Proof. intros Hle Hvα; eapply shift_preserves_wf_gen; eauto. Qed.
 
@@ -234,31 +233,44 @@ End Typ.
 
 (** * Syntax - Pair of types 
 
-  The resource context defined in [RContext.v] maps resource names to pair types. We define it co-domain here. Thanks to the [DeBrLevel] library, we do not have to prove properties that handle level because [PairLevel] already exists.
+  The resource context defined in [RContext.v] maps resource names to pair types. We define it co-domain here.
 *)
 
 
 (** ** Module - Pair of types *)
 Module PairTyp <: IsBdlLvlETWL.
   
-Definition t : Type := Typ.t * Typ.t.
+(** *** Definitions *)
+
+(** **** A pair of types *)
+Definition t: Type := Typ.t * Typ.t.
 Definition eq := @Logic.eq t.
 
-#[export] Instance eq_equiv : Equivalence eq := _.
+#[export] Instance eq_equiv: Equivalence eq := _.
 
+(** **** The shift function 
 
-Definition shift (m n : resource) (tp : t) :=
+  It applies the shift function defined in [Typ] module on both elements of the pair.
+*)
+Definition shift (m n: resource) (tp: t) :=
   let (p1,p2) := tp in 
   (Typ.shift m n p1,Typ.shift m n p2).
 
-Definition Wf (m : resource) (tp : t) :=
+(** **** The well-formed property 
+
+  A pair of types [tp] is well-formed under a level [m] if both types are well-formed under [m].
+*)
+Definition Wf (m: resource) (tp: t) :=
   let (p1,p2) := tp in 
   Typ.Wf m p1 /\ Typ.Wf m p2.
 
+(** *** Properties *)
 
-#[export] Hint Resolve eq_refl eq_sym eq_trans : core.
+(** **** [eq] properties *)
 
-Lemma eq_dec (t1 t2: t) : {eq t1 t2} + {~ eq t1 t2}.
+#[export] Hint Resolve eq_refl eq_sym eq_trans: core.
+
+Lemma eq_dec (t1 t2: t): {eq t1 t2} + {~ eq t1 t2}.
 Proof.
   unfold eq.
   destruct t1 as [p1 p2];
@@ -270,20 +282,20 @@ Proof.
   intro c; inversion c; contradiction.
 Qed.
 
-Lemma eq_leibniz (t1 t2: t) : eq t1 t2 -> t1 = t2. 
+Lemma eq_leibniz (t1 t2: t): eq t1 t2 -> t1 = t2. 
 Proof. auto. Qed.
 
 (** **** [shift] properties *)
 
-Lemma shift_zero_refl (lb : lvl) (t : t) : shift lb 0 t = t.
+Lemma shift_zero_refl (lb: lvl) (t: t): shift lb 0 t = t.
 Proof.
   destruct t as [p1 p2]; simpl.
   now do 2 rewrite Typ.shift_zero_refl.
 Qed.
 
-#[export] Instance shift_eq : Proper (Logic.eq ==> Logic.eq ==> eq ==> eq) shift := _.
+#[export] Instance shift_eq: Proper (Logic.eq ==> Logic.eq ==> eq ==> eq) shift := _.
 
-Lemma shift_eq_iff (lb k : lvl) (t t1 : t) :
+Lemma shift_eq_iff (lb k: lvl) (t t1: t) :
   t = t1 <-> (shift lb k t) = (shift lb k t1).
 Proof.
   split; intro Heq.
@@ -296,21 +308,21 @@ Proof.
     reflexivity.
 Qed.
 
-Lemma shift_trans (lb k m : lvl) (t : t) :
+Lemma shift_trans (lb k m: lvl) (t: t) :
   shift lb k (shift lb m t) = shift lb (k + m) t.
 Proof.
   destruct t as [p1 p2]; simpl.
   now do 2 rewrite Typ.shift_trans.
 Qed.
 
-Lemma shift_permute (lb k m : lvl) (t : t) :
+Lemma shift_permute (lb k m: lvl) (t: t) :
   shift lb k (shift lb m t) = shift lb m (shift lb k t).
 Proof.
   destruct t as [p1 p2]; simpl.
   now f_equal; rewrite Typ.shift_permute.
 Qed.
 
-Lemma shift_permute_1 (lb k m : lvl) (t : t) :
+Lemma shift_permute_1 (lb k m: lvl) (t: t) :
   (shift lb k (shift lb m t)) = (shift (lb + k) m (shift lb k t)).
 Proof.
   destruct t as [p1 p2]; simpl.
@@ -318,7 +330,7 @@ Proof.
   now rewrite Typ.shift_permute_1.
 Qed.
 
-Lemma shift_permute_2 (lb k m n : lvl) (t : t) :
+Lemma shift_permute_2 (lb k m n: lvl) (t: t) :
   lb <= k -> (shift lb m (shift k n t)) = (shift (k + m) n (shift lb m t)).
 Proof.
   intro Hle.
@@ -326,14 +338,14 @@ Proof.
   f_equal; rewrite Typ.shift_permute_2; auto.
 Qed.
 
-Lemma shift_unfold (lb k m : lvl) (t : t) :
+Lemma shift_unfold (lb k m: lvl) (t: t) :
   (shift lb (k + m) t) = (shift (lb + k) m (shift lb k t)). 
 Proof.
   destruct t as [p1 p2]; simpl.
   f_equal; now rewrite Typ.shift_unfold.
 Qed.
 
-Lemma shift_unfold_1 (k m n : lvl) (t : t) :
+Lemma shift_unfold_1 (k m n: lvl) (t: t) :
   k <= m -> m <= n -> 
   (shift m (n - m) (shift k  (m - k) t)) = (shift k (n - k) t).
 Proof.
@@ -342,7 +354,7 @@ Proof.
   f_equal; rewrite Typ.shift_unfold_1; auto.
 Qed.
 
-Lemma shift_wf_refl m k t : Wf m t -> (shift m k t) = t.
+Lemma shift_wf_refl m k t: Wf m t -> (shift m k t) = t.
 Proof.
   destruct t as [p1 p2]; simpl.
   intros [Hwf1 Hwf2].
@@ -351,9 +363,9 @@ Qed.
 
 (** **** [Wf] properties *)
 
-#[export] Instance Wf_iff : Proper (Logic.eq ==> eq ==> iff) Wf := _.
+#[export] Instance Wf_iff: Proper (Logic.eq ==> eq ==> iff) Wf := _.
 
-Lemma Wf_weakening (k m : lvl) (t : t) : (k <= m) -> Wf k t -> Wf m t.
+Lemma Wf_weakening (k m: lvl) (t: t): (k <= m) -> Wf k t -> Wf m t.
 Proof.
   unfold Wf.
   destruct t as [p1 p2].
@@ -361,7 +373,7 @@ Proof.
   split; eapply Typ.Wf_weakening; eauto.
 Qed.
 
-Theorem shift_preserves_wf_1 (lb k m : lvl) (t : t) :
+Theorem shift_preserves_wf_1 (lb k m: lvl) (t: t) :
   Wf k t -> Wf (k + m) (shift lb m t).
 Proof.
   unfold Wf.
@@ -371,11 +383,11 @@ Proof.
   split; now apply Typ.shift_preserves_wf_1.
 Qed.
 
-Theorem shift_preserves_wf (k m : lvl) (t : t) :
+Theorem shift_preserves_wf (k m: lvl) (t: t) :
   Wf k t -> Wf (k + m) (shift k m t).
 Proof. intros; now apply shift_preserves_wf_1. Qed. 
 
-Theorem shift_preserves_wf_zero (k : lvl) (t : t) :
+Theorem shift_preserves_wf_zero (k: lvl) (t: t) :
   Wf k t -> Wf k (shift k 0 t).
 Proof. 
   unfold Wf.
@@ -385,7 +397,7 @@ Proof.
   split; now apply Typ.shift_preserves_wf_zero.
 Qed. 
 
-Lemma shift_preserves_wf_gen (lb k m n : lvl) (t : t) :
+Lemma shift_preserves_wf_gen (lb k m n: lvl) (t: t) :
     m <= n -> lb <= k -> m <= lb -> n <= k -> n - m = k - lb -> 
     Wf lb t -> Wf k (shift m (n - m) t).
 Proof.
@@ -397,7 +409,7 @@ Proof.
   split; apply Typ.shift_preserves_wf_gen with (lb := lb); auto.
 Qed.
 
-Lemma shift_preserves_wf_2 (m n : lvl) (t : t) :
+Lemma shift_preserves_wf_2 (m n: lvl) (t: t) :
   m <= n -> Wf m t -> Wf n (shift m (n - m) t).
 Proof. 
   intros Hle Hvt. 
@@ -429,26 +441,26 @@ Notation "t1 '×' t2"   := (Typ.ty_prod t1 t2)
 Notation "t1 '⟿' t2 '∣' R" := (Typ.ty_reactive t1 t2 R)
                                (in custom wh at level 50, R constr, right associativity).
 Notation "'[⧐' lb '–' k ']' t" := (Typ.shift lb k t) 
-                                   (in custom wh at level 45, right associativity) : typ_scope.
+                                   (in custom wh at level 45, right associativity): typ_scope.
 Notation "'[⧐⧐' lb '–' k ']' t" := (Typ.multi_shift lb k t) 
-                                    (in custom wh at level 45, right associativity) : typ_scope.
+                                    (in custom wh at level 45, right associativity): typ_scope.
 Notation "'[⧐' lb '–' k ']' t" := (PairTyp.shift lb k t) 
-                                   (in custom wh at level 45, right associativity) : ptyp_scope.
+                                   (in custom wh at level 45, right associativity): ptyp_scope.
 
 Infix "⊩"  := Typ.Wf (at level 20, no associativity): typ_scope. 
-Infix "⊩"  := PairTyp.Wf (at level 20, no associativity) : ptyp_scope. 
-Infix "="  := Typ.eq : typ_scope.
+Infix "⊩"  := PairTyp.Wf (at level 20, no associativity): ptyp_scope. 
+Infix "="  := Typ.eq: typ_scope.
 
 (** *** Morphisms *)
 Import Typ.
 
-#[export] Instance typ_leibniz_eq : Proper Logic.eq Typ.eq := _.
+#[export] Instance typ_leibniz_eq: Proper Logic.eq Typ.eq := _.
 
-#[export] Instance typ_wf_iff :  Proper (Level.eq ==> eq ==> iff) Wf := _.
+#[export] Instance typ_wf_iff:  Proper (Level.eq ==> eq ==> iff) Wf := _.
 
-#[export] Instance typ_shift_eq : Proper (Level.eq ==> Level.eq ==> eq ==> eq) shift := shift_eq.
+#[export] Instance typ_shift_eq: Proper (Level.eq ==> Level.eq ==> eq ==> eq) shift := shift_eq.
 
-#[export] Instance typ_multi_shift_eq : 
+#[export] Instance typ_multi_shift_eq: 
   Proper (Logic.eq ==> Logic.eq ==> eq ==> Logic.eq) multi_shift := _.
 
 End TypNotations.
