theories/Syntax/Var.v
@@ -3,7 +3,7 @@ From DeBrLevel Require Import LevelInterface.
 
 (** * Syntax - Variable
 
-  We represent variables with [nat]. 
+  In our mechanization, a variable is a [nat]. Consequently we use [Nat_as_OT] in order to represent the countable infinite set of variables.  
 *)
 
 (** ** Module - Variable *)
@@ -11,7 +11,7 @@ Module Var <: OrderedTypeWithLeibniz.
 
 Include Nat_as_OT.
 
-Lemma eq_leibniz (x y: t): eq x y -> x = y. 
+Lemma eq_leibniz (x y: t) : eq x y -> x = y. 
 Proof. auto. Qed.
 
 End Var.
